![[Pasted image 20230928220942.png]]
### 19.13

![[Pasted image 20230928214439.png]]
![[Pasted image 20230928222208.png]]
$y_1 =0,2; m=13$
![[Pasted image 20230928222321.png]]
### 19.17
![[Pasted image 20230928224636.png]]
Поступаем аналогично предыдущей задаче
$y_1 =0,2; m=13$
![[Pasted image 20230928223454.png]]
$F^{-1} = a-\sqrt{2*\sigma^2 * ln(\sigma*\sqrt{2*\pi}*y_i)}$

![[Pasted image 20230928225711.png]]

### 19.19

![[Pasted image 20230928231802.png]]
Поступаем аналогично предыдущей задаче
$y_1 =0,2; m=13$

![[Pasted image 20230928231112.png]]
Получим обратные:
- Для X: $F^{-1} = a+\sigma*\sqrt{-2*ln(y_{i-1})}*cos(2*\pi*y_i)$
- Для Y: $F^{-1} = a+\sigma*\sqrt{-2*ln(y_{i-1})}*sin(2*\pi*y_i)$


![[Pasted image 20230928233625.png]]





